spinlock adequacy

examples/spinlock/SpinLockAll.v
@@ -5,10 +5,54 @@ Require Import SpinLockMainHeader SpinLockMainI SpinLockMainA SpinLockMainIAProo
 Require Import SchHeader SchI SchA SchIAproof.
 Require Import ElimRel SModCancel Cancellation.
 
-Module IncrAll.
-  Import inv_instances.
+(* From iris Require Import frac_auth numbers. *)
+Module SpinLockAll.
+  Local Existing Instances invG_Σ invG_Γ invG_I invG_E invG_D.
+
+  Instance τ : TypG.t := λ _, ST.t.
+  Instance typG : CtxST.t τ. Proof. econs. econs. instantiate (1:=0); ss. Qed.
+
   Local Instance Γ : HRA := ##[invΓ; memΓ; SchAΓ; SpinLockΓ; SpinLockMainAΓ].
+  Local Instance α : SRFCons.t :=
+    λ n,
+      match n with
+      | 0 => SL.syntax
+      | _ => inv_syntax
+      end.
   Local Instance Σ : GRA := ##[invΣ; SchAΣ; Γ].
+  Local Instance sub : subG Γ Σ.
+  Proof. do 2 apply subG_app_r. apply subG_refl. Defined.
+  Local Instance invG : invG α Σ Γ.
+  Proof. econs. { econs. exists 0%fin. ss. } { econs. { exists 0%fin. ss. } { exists 1%fin. ss. } } Defined.
+  Instance β : SRFIntp.t :=
+    λ n,
+      match n with
+      | 0 => SL.interp
+      | _ => inv_interp
+      end.
+  Local Instance intpG : SRFIntp.inG (@SL.syntax τ Γ) α (@SL.interp τ α Γ Σ _) β.
+  Proof. econs; instantiate (1:=0); ss. Qed.
+
+  Local Instance invintpG : SRFIntp.inG inv_syntax α inv_interp β.
+  Proof. econs; instantiate (1:=1); ss. Qed.
+
+  Local Instance sinvg : sinvG Σ Γ α β τ.
+  Proof. econs; econs; try typeclasses eauto. Qed.
+
+  Local Instance memΓ : memGΓ Γ.
+  Proof. econs. exists 2%fin; ss. Defined.
+
+  Local Instance SchAΓ : SchAGΓ Γ.
+  Proof. econs. exists 3%fin; ss. Defined.
+
+  Local Instance SpinLockAGΓ : SpinLockAGΓ Γ.
+  Proof. econs. exists 4%fin; ss. Defined.
+
+  Local Instance SpinLockMainAGΓ : SpinLockMainAGΓ Γ.
+  Proof. econs. exists 5%fin; ss. Defined.
+
+  Local Instance SchAΣ : SchAGΣ Σ.
+  Proof. econs. exists 1%fin; ss. Defined.
 
   (* building the target module *)
   Local Definition csl : string → bool := λ _, false.
@@ -43,17 +87,18 @@ Module IncrAll.
   Proof.
     apply ctxr_refines.
     rewrite /mod_src /smod_src /mod_tgt /init_cond ?add_interp_comm.
+    replace (SMod.to_hmod _ _ (SpinLockMainA.Mod _)) with (SpinLockMainA.t u spc_s); cycle 1.
+    { unfold_hmod; ss. }
+    replace (SMod.to_hmod _ _ (MemA.Mod)) with (MemA.t u spc_s); cycle 1.
+    { unfold_hmod; ss. }
+    replace (SMod.to_hmod _ _ (SpinLockA.Mod _)) with (SpinLockA.t u spc_s); cycle 1.
+    { unfold_hmod; ss. }
+
     etrans.
     { do 2 eapply ctxr_frameL. eapply ctxr_comm. }
     do 2 rewrite -hmod_add_assoc.
     etrans.
     { eapply ctxr_frameR.
-      replace (SMod.to_hmod _ _ (SpinLockMainA.Mod _)) with (SpinLockMainA.t u spc_s); cycle 1.
-      { unfold_hmod; ss. }
-      replace (SMod.to_hmod _ _ (MemA.Mod)) with (MemA.t u spc_s); cycle 1.
-      { unfold_hmod; ss. }
-      replace (SMod.to_hmod _ _ (SpinLockA.Mod _)) with (SpinLockA.t u spc_s); cycle 1.
-      { unfold_hmod; ss. }
       rewrite hmod_add_assoc -hmod_addc_empty_l.
       etrans; first eapply ctxr_cond_frameR.
       { eapply SpinLockMainIA.wctxr; eauto.
@@ -85,7 +130,7 @@ Module IncrAll.
     rewrite hmod_add_assoc.
     etrans; first eapply ctxr_comm. rewrite -hmod_add_assoc. eapply ctxr_frameR.
     etrans.
-    { rewrite hmod_addc_empty_l. eapply ctxr_frameR, ctxr_cond_frameR. eapply MemIA.correct.
+    { rewrite hmod_addc_empty_l. eapply ctxr_frameR, ctxr_cond_frameR. eapply MemIA.wctxr.
       rewrite /MemA.Spc; unseal CRIS.
       split; first prove_nodup. ii; ss; des_ifs; rewrite ->eq_rel_dec_correct in *; des_ifs.
     }
@@ -105,136 +150,53 @@ Module IncrAll.
     refl.
   Qed.
 
-  Local Definition initial_resource : Σ :=
-    own_admin MainAS.init_res ⋅ CannonAS.init_res.
-
-(* 
-  Local Definition SchInSpc : ∀ u, spc_incl (SchAS.spc u (spc_user_s u)) (spc_s u).
-  Proof.
-    ii; rewrite /spc_s /SchAS.spc /MemA.Spc /IncrMainAS.spc; unseal CRIS; split; [prove_nodup|ii].
-    ss; des_ifs; rewrite ->eq_rel_dec_correct in *; des_ifs.
-  Qed.
-  Local Definition MainInSpc : ∀ u, spc_incl (IncrMainAS.spc u) (spc_user_s u).
-  Proof.
-    ii; rewrite /spc_s /SchAS.spc /MemA.Spc /IncrMainAS.spc; unseal CRIS; split; [prove_nodup|ii].
-    ss; des_ifs; rewrite ->eq_rel_dec_correct in *; des_ifs.
-  Qed.
-  Local Definition MemInSpc : ∀ u, spc_incl MemA.Spc (spc_s u).
-  Proof.
-    ii; rewrite /spc_s /SchAS.spc /MemA.Spc /IncrMainAS.spc; unseal CRIS; split; [prove_nodup|ii].
-    ss; des_ifs; rewrite ->eq_rel_dec_correct in *; des_ifs.
-  Qed.
-
-  (* Local Definition ctxr := (IncrIA.wctxr ginv spc_s spc_user_s spc_s SchInSpc MainInSpc MemInSpc).
-
-  Local Definition k := proj1_sig ctxr.
-  Local Definition k_prf := proj2_sig ctxr.
-  Local Definition u : nat := k.
-  Local Definition v : nat := 0.
-
-  Local Definition csl : string → bool := λ _, false.
-  Local Definition genv : GEnv.t := GEnv.unit.
-
-  Local Definition smod_src : SMod.t := 
-    (IncrMainA.Mod u) ☆ (MemA.Mod) ☆ (SchA.Mod u (spc_user_s u)).
-  Local Definition smod_cancel : HMod.t := SModCancel.to_hmod smod_src.
-  Local Definition mod_src : HMod.t := SMod.to_hmod (ginv u) (spc_s u) smod_src.
-  Local Definition mod_tgt : HMod.t := IncrMainI.t ★ (MemI.t csl genv) ★ (SchI.t). *)
-
-  Local Definition init_cond : iProp Σ := MemA.InitCond csl genv ∗ SchA.InitCond.
-  Local Definition main_fsp : univ_id → fspec := λ u, IncrMainAS.main_spec u.
-
-  (* Apply cancellation to linked spec module *)
-  Lemma cancel_src :
-    ∀ u,
-      refines (smod_cancel u, (init_cond ∗ (main_fsp u).(precond) 0 tt tt↑ tt↑)%I) 
-              (mod_src u, init_cond).
-  Proof. i; eapply cancellation; try by econs. i. iIntros "[_ %POST]". iPureIntro. des; eauto. Qed.
-
-  (* Refinement between spec/impl of whole program (linked module) *)
-  Lemma src_tgt : ∃ k, refines (mod_src k, init_cond) (mod_tgt, emp%I).
-  Proof.
-    hexploit (IncrIA.wctxr ginv spc_s spc_user_s spc_s); eauto using SchInSpc, MainInSpc, MemInSpc.
-    intros [k k_prf]; exists (k + 1).
-    eapply ctxr_refines.
-    rewrite -[(mod_src (k + 1), _)]hmod_addc_empty_l.
-    rewrite -[(mod_tgt, _)]hmod_addc_empty_r.
-    rewrite /mod_src /mod_tgt ?add_interp_comm /init_cond.
-    rewrite -hmod_add_assoc. rewrite -hmod_add_assoc. rewrite assoc. eapply ctxr_compose_hor.
-    { etrans.
-      { eapply ctxr_cond_frameR.
-        replace (SMod.to_hmod _ _ (IncrMainA.Mod (k + 1))) with (IncrMainA.t (k + 1) (ginv (k + 1)) (spc_s (k + 1))); cycle 1.
-        { rewrite /IncrMainA.t; unseal CRIS; ss. }
-        replace (SMod.to_hmod _ _ (MemA.Mod)) with (MemA.t (ginv (k + 1)) (spc_s (k + 1))); cycle 1.
-        { rewrite /MemA.t; unseal CRIS; ss. }
-        eapply (k_prf _ 1); lia.
-      }
-      { eapply ctxr_frameL. etrans; first eapply ctxr_cond_frameL, MemIA.correct.
-        { eauto using MemInSpc. }
-        { eapply ctxr_cond_strengthen; eauto. }
-      }
-    }
-    eapply main_adequacy.
-    replace (SMod.to_hmod _ _ (SchA.Mod (k + 1) (spc_user_s (k + 1)))) with (SchA.t (k + 1) (spc_s (k + 1)) (spc_user_s (k + 1))); cycle 1.
-    { rewrite /SchA.t; unseal CRIS; ss. }
-    eapply SchIA.sim; eauto using SchInSpc.
-    { rewrite /spc_sub /spc_user_s /spc_s /IncrMainAS.spc /MemA.Spc; unseal CRIS. ii; ss.
-      des_ifs; rewrite ->eq_rel_dec_correct in *; des_ifs.
-    }
-  Qed.
-
   Lemma cancel_tgt :
-    ∃ u,
-    refines (smod_cancel u, (init_cond ∗ (main_fsp u).(precond) 0 tt tt↑ tt↑)%I)
+    refines (smod_cancel, (init_cond ∗ (main_fsp).(precond) tt tt↑ tt↑)%I)
             (mod_tgt, emp%I).
   Proof.
-    pose proof src_tgt as [k H]; exists k.
     etrans.
     { eapply cancel_src. }
-    { done. }
+    { eapply src_tgt. }
   Qed.
 
-  Local Definition initial_resource : Σ :=
-    (MemA.mem_init_res csl genv) ⋅ SchAS.initial_resource.
+  Import rListNotations.
+  Local Definition initial_resource_list : res_list :=
+    [ownIRA_resource u; ownERA_resource u; ownDRA_resource u;
+     SchAS.tidRA_resource; SchAS.threadsRA_resource; memRA_resource csl genv]%res_list.
+
+  Local Definition initial_resource : Σ := 
+    (op_res_list initial_resource_list) ⋅ initial_resource_own_admin.
+
+  Ltac dfs_solve :=
+    econs; [repeat (intros [C | C]; [inv C|]; revert C); intros []|].
+    
   Lemma initial_resource_valid : ✓ initial_resource.
   Proof.
-    dfs_unfold; dfs_merge; dfs_to_list; dfs_resolve.
-    { rewrite /SchAΣ in x.
-      rewrite inG_id_subG_inG in x.
-      inv_instances.solve_in_subG_goal.
-      rewrite ?/eq_rec_r ?/eq_rec in x; try rewrite -!eq_rect_eq in x; ss; eauto.
-    }
-    { dfs_split; dfs_simplify.
-      { pose proof mem_initial_valid csl genv. eapply cmra_valid_op_l; eauto. }
-      { rewrite /SchAS.initial_threads_r; eapply auth_both_valid_discrete; split.
-        { exists (λ tid, if (tid =? 0) then Some ((3/4)%Qp, to_agree (λ _ : SAny.t, Some (to_agree (existT 0 ⊤%SRF)))) else None).
-          intros i; des_ifs; ss; [rewrite Nat.eqb_eq in Heq|rewrite Nat.eqb_neq in Heq]; clarify; ss.
-          { rewrite discrete_fun_lookup_op //= -Some_op -pair_op frac_op; repeat f_equiv; ss.
-            { rewrite Qp.quarter_three_quarter; ss. }
-            { rr; ii; split; ii; esplits; eauto; try set_solver. }
-          }
-          { rewrite discrete_fun_lookup_op; des_ifs; rewrite Nat.eqb_eq in Heq0; ss. }
-        }
-        { ii; des_ifs; ss. }
-      }
-    }
+    apply op_res_list_valid.
+    repeat dfs_solve. econs.
   Qed.
 
   Theorem behavioral_refinement :
-    ∃ u target_resource, refines_mod
-      (HMod.to_mod (smod_cancel u) initial_resource)
+    ∃ target_resource, refines_mod
+      (HMod.to_mod smod_cancel initial_resource)
       (HMod.to_mod mod_tgt target_resource).
   Proof.
-    move: (cancel_tgt)=>[u H]; rewrite /refines in H; ss; exists u.
+    move: (cancel_tgt)=>H; rewrite /refines in H; ss.
     destruct (H initial_resource).
     { apply initial_resource_valid. }
-    { iIntros "[M S]".
-      rewrite /init_cond /MemA.InitCond /SchA.InitCond /precond /main_fsp /IncrMainAS.main_spec; ss.
-      rewrite /precond /fspec_simple /=.
-      admit.
+    { iIntros "H". iPoseProof (big_bang with "H") as "[O H]".
+      iDestruct "H" as "[H1 [H2 [H3 [H4 [H5 [H6 _]]]]]]"; iFrame.
+      iPoseProof (ownI_initial_gen with "[$]") as "[U W]".
+      iPoseProof (SchAS.tid_admin_none_split with "[H4]") as "[H3 H4]".
+      { rewrite /SchAS.tid_admin; unseal "SchA"; ss. }
+      iFrame. des_ifs. unfold_pre_post. iSplitL.
+      { iSplitR "H5".
+        { iDestruct "H6" as "[$ $]". }
+        { rewrite /SchAS.initial_threads. unseal "SchA". done. }
+      }
+      iSplit; eauto.
     }
-    { econs; ss; try prove_nodup. }
+    { econs; ss; prove_nodup. }
     { exists x; des; eauto. }
-  Admitted. *)
-End IncrAll.
-(* Print Assumptions CannonAll.behavioral_refinement. *)
+  Qed.
+End SpinLockAll.
