theories/iris_system/own.v
@@ -46,7 +46,7 @@ Definition own_admin := own_admin_aux.(unseal).
 Local Definition own_admin_eq : @own_admin = @own_admin_def := own_admin_aux.(seal_eq).
 Global Arguments own_admin {_}.
 Definition initial_resource_own_admin {Σ : GRA} : GRAUR Σ :=
-  λ i, allocs_auth (@GRA_lookup Σ i) (λ x, x <> base_γ).
+  λ i, allocs_auth (@GRA_lookup Σ i) (.∈ (⊤ ∖ {[base_γ]} : coPset)).
 
 (** * Definitions of resource ownership - for metatheoretical uses only *)
 Local Definition Own_def {Σ : GRA} (a : Σ) : iProp Σ := uPred_ownM a.
@@ -401,28 +401,46 @@ Section Own.
   Qed.
 
 End Own.
-(* 
+
 Definition resource {Σ : GRA} (A : cmra) : Type := { a : A & inG A Σ & ✓ a}.
+
 Inductive res_list {Σ : GRA} :=
 | r_nil
 | r_cons (A : cmra) (r : resource A) (l : res_list).
+
+Declare Scope rlist_scope.
+Delimit Scope rlist_scope with res_list.
+Bind Scope rlist_scope with res_list.
+
+Infix "::" := (r_cons _) (at level 60, right associativity) : rlist_scope.
+Module rListNotations.
+Notation "[ ]" := r_nil (format "[ ]") : rlist_scope.
+Notation "[ x ]" := (r_cons _ x r_nil) : rlist_scope.
+Notation "[ x ; y ; .. ; z ]" :=  (r_cons _ x (r_cons _ y .. (r_cons _ z r_nil) ..))
+  (format "[ '[' x ;  '/' y ;  '/' .. ;  '/' z ']' ]") : rlist_scope.
+End rListNotations.
+
 Definition eq_index {Σ : GRA} {A B} (a : resource A) (b : resource B) : Prop.
 Proof. destruct a as [a [ia va]]. destruct b as [b [ib vb]]. exact (ia = ib). Defined.
-Fixpoint In {Σ : GRA} {A} (a : resource A) (l : res_list) : Prop :=
+
+Fixpoint r_In {Σ : GRA} {A} (a : resource A) (l : res_list) : Prop :=
   match l with
     | r_nil => False
-    | r_cons B b tl => eq_index a b ∨ In a tl
+    | r_cons B b tl => eq_index a b ∨ r_In a tl
   end.
-Inductive NoDup {Σ : GRA} : res_list → Prop :=
-| NoDup_nil : NoDup r_nil
-| NoDup_cons : forall X (x : resource X) l, ~ In x l → NoDup l → NoDup (r_cons _ x l).
+
+Inductive r_NoDup {Σ : GRA} : res_list → Prop :=
+| r_NoDup_nil : r_NoDup r_nil
+| r_NoDup_cons : forall X (x : resource X) l, ~ r_In x l → r_NoDup l → r_NoDup (r_cons _ x l).
+
 Fixpoint op_res_list {Σ : GRA} (l : res_list) : Σ :=
   match l with
   | r_nil => ε
   | r_cons A (existT2 _ _ a inG V) tl => (iRes_singleton base_γ a) ⋅ (op_res_list tl)
   end.
+
 Lemma not_in_emp {Σ : GRA} {R} (r : resource R) (l : res_list) :
-  ~ In r l → (op_res_list l (inG_id (projT2 (sigT_of_sigT2 r)))) ≡ ε.
+  ~ r_In r l → (op_res_list l (inG_id (projT2 (sigT_of_sigT2 r)))) ≡ ε.
 Proof.
   revert r. induction l; first ss.
   intros r0 NIN. destruct r0 as [r0 [in0 v0]]. destruct r as [r1 [in1 v1]].
@@ -436,19 +454,28 @@ Proof.
     { ii; clarify. }
   }
 Qed.
-(* TODO : own_admin *)
-Lemma op_res_list_valid {Σ : GRA} (l : res_list) (NODUP : NoDup l) : ✓ (op_res_list l).
+Lemma op_res_list_valid {Σ : GRA} (l : res_list) (NODUP : r_NoDup l) :
+  ✓ (op_res_list l ⋅ initial_resource_own_admin).
 Proof.
-  induction l; ss. inv NODUP. inv H0. clear r H2. destruct x0 as [r [ING VALID]].
+  induction l; ss.
+  { rewrite left_id /initial_resource_own_admin; intros i.
+    rewrite /allocs_auth; intros k; des_ifs.
+  }
+  inv NODUP. inv H0. clear r H2. destruct x0 as [r [ING VALID]].
   intros i; rewrite discrete_fun_lookup_op.
   destruct (decide (i = ING)).
   { hexploit (@not_in_emp _ A).
     { ii; eapply H1; eapply H. }
-    ss. rewrite e. intros ->; ss. rewrite right_id.
-    rewrite /iRes_singleton /= discrete_fun_lookup_singleton allocs_frag_valid cmra_transport_valid.
-    done.
+    ss. rewrite e discrete_fun_lookup_op. intros ->; ss. rewrite right_id.
+    rewrite /initial_resource_own_admin /allocs_auth; intros k; rewrite discrete_fun_lookup_op.
+    des_ifs.
+    { rewrite /iRes_singleton /= discrete_fun_lookup_singleton.
+      rewrite /allocs_frag discrete_fun_lookup_singleton_ne //. set_solver.
+    }
+    rewrite right_id /iRes_singleton /= discrete_fun_lookup_singleton.
+    by eapply allocs_frag_valid.
   }
-  rewrite /iRes_singleton discrete_fun_lookup_singleton_ne; ss; last ii; clarify.
+  rewrite discrete_fun_lookup_op /iRes_singleton /= discrete_fun_lookup_singleton_ne //.
   rewrite left_id. apply IHl; eauto.
 Qed.
 Definition own_res_list {Σ : GRA} (l : res_list) : iProp Σ.
@@ -457,55 +484,17 @@ Proof.
   { exact True%I. }
   { destruct b as [b [ib va]]. refine (@own B Σ (inG_mk B Σ ib va) base_γ b ∗ IHtl)%I. }
 Defined.
-Lemma big_bang {Σ : GRA} (l : res_list) : Own (op_res_list l) ⊢ own_admin ∗ own_res_list l.
+Lemma big_bang {Σ : GRA} (l : res_list) :
+  Own (op_res_list l ⋅ initial_resource_own_admin) ⊢ own_admin ∗ own_res_list l.
 Proof.
-  induction l; first iIntros "_ //".
-  destruct r as [r [IN VAL]]; iIntros "[O1 O2] /=".
-  iSplitL "O1".
-  { rewrite own_eq /own_def Own_eq /Own_def //. }
-  { iApply IHl; iFrame. }
+  induction l; first iIntros "[_ O] //".
+  { iSplitL; ss. rewrite own_admin_eq /own_admin_def; iExists (⊤ ∖ {[base_γ]}).
+    iSplit.
+    { iPureIntro. eapply difference_infinite, singleton_finite. eapply top_infinite. }
+    { rewrite /initial_resource_own_admin Own_eq /Own_def. iFrame. }
+  }
+  destruct r as [r [IN VAL]]; iIntros "[[O1 O3] O2] /=".
+  iPoseProof (IHl with "[O3 O2]") as "[$ $]".
+  { iSplitL "O3"; iFrame. }
+  rewrite Own_eq /Own_def own_eq /own_def //.
 Qed.
-From iris Require Import excl auth.
-Class MapMGΓ (Γ : GRA) := {
-  #[local] map_inG :: inG (exclR unitO) Γ;
-}.
-Definition MapMΓ : GRA := #[exclR unitO].
-Global Instance subG_GΓ {Γ : GRA} : subG MapMΓ Γ → MapMGΓ Γ.
-Proof. solve_inG. Defined.
-Hint Unfold subG_GΓ map_inG : GRA_index.
-
-Local Definition RA : ucmra :=
-  prodUR (optionUR (exclR unitO)) (authUR (Z -d> optionUR (exclR ZO))).
-Class MapAGΓ (Γ : GRA) := { #[local] RA_inG :: inG RA Γ }.
-Definition MapAΓ : GRA := #[RA].
-Global Instance AsubG_GΓ {Γ : GRA} : subG MapAΓ Γ → MapAGΓ Γ.
-Proof. solve_inG. Defined.
-Hint Unfold AsubG_GΓ MapAΓ : GRA_index.
-Section user.
-  Context `{!MapMGΓ Σ, !MapAGΓ Σ}.
-  Program Definition initial_resource : resource (exclR unitO) :=
-    existT2 _ _ (Excl ()) _ _.
-  Next Obligation. ss. apply _. Defined.
-  Next Obligation. ss. Defined.
-
-  Program Definition initial_resource_A : resource RA :=
-    existT2 _ _ (Some (Excl ()), ε) _ _.
-  Next Obligation. ss. apply _. Defined.
-  Next Obligation. ss. eapply pair_valid; split; ss. eapply ucmra_unit_valid. Defined.
-  Definition init_cond : iProp Σ := own base_γ (Excl ()) ∗ own base_γ (Some (Excl ()), ε).
-End user.
-
-Section big_bang.
-  Local Instance Σ : GRA := ##[MapMΓ; MapAΓ].
-  Lemma cancel : ∃ rs, ✓ rs ∧ (Own rs ⊢ init_cond).
-  Proof.
-    exists (op_res_list (r_cons _ initial_resource_A (r_cons _ initial_resource r_nil))). split.
-    { apply op_res_list_valid. rewrite /initial_resource. econs; ss; cycle 1.
-      { econs; ss. econs; ss. }
-      rewrite /initial_resource_obligation_2 /initial_resource_A_obligation_2. ss.
-      ii; des; ss. admit. }
-    { iIntros "O". iPoseProof (big_bang with "O") as "O".
-      rewrite /init_cond. ss. des_ifs. iDestruct "O" as "[$ [$ _]]".
-    }
-  Qed.
-   *)
